ulib/experimental/Steel.Heap.fsti
@@ -523,12 +523,15 @@ val change_slprop (p q:slprop)
 
 module U = FStar.Universe
 
-val lift_h_exists (#a:_) (p:a -> slprop)
-  : action (h_exists p) unit
-           (fun _a -> h_exists #(U.raise_t a) (U.lift_dom p))
+(** Implication of slprops *)
+let slimp (p1 p2:slprop) : prop =
+  forall m. interp p1 m ==> interp p2 m
 
-val elim_pure (p:prop)
-  : action (pure p) (u:unit{p}) (fun _ -> emp)
+let is_frame_monotonic #a (p : a -> slprop) : prop =
+  forall x y m frame. interp (p x `star` frame) m /\ interp (p y) m ==> slimp (p x) (p y)
+
+let witness_invariant #a (p : a -> slprop) =
+  forall x y m. interp (p x) m /\ interp (p y) m ==> x == y
 
 val id_elim_star (p q:slprop) (h:heap)
   : Pure (erased heap & erased heap )
@@ -542,6 +545,17 @@ val id_elim_exists (#a:Type) (p : a -> slprop) (h:heap)
   : Pure (erased a)
          (requires (interp (h_exists p) h))
          (ensures (fun x -> interp (p x) h))
+
+
+val witness_h_exists (#a:_) (p:a -> slprop{is_frame_monotonic p})
+  : action (h_exists p) (erased a) (fun x -> p x)
+
+val lift_h_exists (#a:_) (p:a -> slprop)
+  : action (h_exists p) unit
+           (fun _a -> h_exists #(U.raise_t a) (U.lift_dom p))
+
+val elim_pure (p:prop)
+  : action (pure p) (u:unit{p}) (fun _ -> emp)
 
 val pts_to_evolve (#a:Type u#a) (#pcm:_) (r:ref a pcm) (x y : a) (h:heap)
   : Lemma (requires (interp (pts_to r x) h /\ compatible pcm y x))
